Weidenbach_Book/IsaSAT/Heaps_Abs.thy
@@ -21,57 +21,64 @@ locale hmstruct_with_prio =
 begin
 
     definition prio_peek_min where
-      "prio_peek_min \<equiv>  (\<lambda>(b, w). (\<lambda>v.
+      "prio_peek_min \<equiv>  (\<lambda>(\<A>, b, w). (\<lambda>v.
           v \<in># b
         \<and> (\<forall>v'\<in>set_mset b. le (w v) (w v'))))"
 
     definition mop_prio_peek_min where
-      "mop_prio_peek_min \<equiv>  (\<lambda>(b, w). doN {ASSERT (b\<noteq>{#}); SPEC (prio_peek_min (b,w))})"
+      "mop_prio_peek_min \<equiv>  (\<lambda>(\<A>, b, w). doN {ASSERT (b\<noteq>{#}); SPEC (prio_peek_min (\<A>, b,w))})"
 
     definition mop_prio_change_weight where
-      "mop_prio_change_weight \<equiv>  (\<lambda>v \<omega> (b, w). doN {
-        RETURN (b, w(v := \<omega>))
+      "mop_prio_change_weight \<equiv>  (\<lambda>v \<omega> (\<A>, b, w). doN {
+        ASSERT (v \<in># \<A>);
+        RETURN (\<A>, b, w(v := \<omega>))
      })"
 
     definition mop_prio_insert where
-      "mop_prio_insert \<equiv>  (\<lambda>v \<omega> (b, w). doN {
-        ASSERT (v \<notin># b);
-        RETURN (add_mset v b, w(v := \<omega>))
+      "mop_prio_insert \<equiv>  (\<lambda>v \<omega> (\<A>, b, w). doN {
+        ASSERT (v \<notin># b \<and>  v\<in>#\<A>);
+        RETURN (\<A>, add_mset v b, w(v := \<omega>))
      })"
 
     definition mop_prio_insert_maybe where
       "mop_prio_insert_maybe \<equiv>  (\<lambda>v \<omega> (bw). doN {
-        if v \<notin># fst bw then mop_prio_insert v \<omega> (bw)
+        if v \<notin># fst (snd bw) then mop_prio_insert v \<omega> (bw)
         else mop_prio_change_weight v \<omega> (bw)
      })"
 
     definition mop_prio_insert_raw_unchanged where
-      "mop_prio_insert_raw_unchanged = (\<lambda>v (b, w). doN {
-        ASSERT (v \<notin># b);
-        RETURN (add_mset v b, w)
+      "mop_prio_insert_raw_unchanged = (\<lambda>v (\<A>, b, w). doN {
+        ASSERT (v \<notin># b \<and> v \<in># \<A>);
+        RETURN (\<A>, add_mset v b, w)
      })"
 
     definition mop_prio_insert_unchanged where
       "mop_prio_insert_unchanged =  (\<lambda>v (bw). doN {
-        if v \<notin># fst bw then mop_prio_insert_raw_unchanged v (bw)
+        if v \<notin># fst (snd bw) then mop_prio_insert_raw_unchanged v (bw)
         else RETURN bw
      })"
 
     definition prio_del where
-      \<open>prio_del = (\<lambda>v (b, w). (b - {#v#}, w))\<close>
+      \<open>prio_del = (\<lambda>v (\<A>, b, w). (\<A>, b - {#v#}, w))\<close>
 
     definition mop_prio_del where
-      "mop_prio_del = (\<lambda>v (b, w). doN {
-        ASSERT (v \<in># b);
-        RETURN (prio_del v (b, w))
+      "mop_prio_del = (\<lambda>v (\<A>, b, w). doN {
+        ASSERT (v \<in># b \<and> v \<in># \<A>);
+        RETURN (prio_del v (\<A>, b, w))
      })"
 
     definition mop_prio_pop_min where
-      "mop_prio_pop_min = (\<lambda>(b, w). doN {ASSERT (b\<noteq>{#});
-      v \<leftarrow> mop_prio_peek_min (b, w);
-      bw \<leftarrow> mop_prio_del v (b, w);
+      "mop_prio_pop_min = (\<lambda>(\<A>, b, w). doN {ASSERT (b\<noteq>{#});
+      v \<leftarrow> mop_prio_peek_min (\<A>, b, w);
+      bw \<leftarrow> mop_prio_del v (\<A>, b, w);
       RETURN (v, bw)
       })"
+
+    definition mop_prio_old_weight where
+      "mop_prio_old_weight = (\<lambda>v (\<A>, b, w). doN {
+        ASSERT (v \<in># \<A>);
+        RETURN (w v)
+     })"
 
 sublocale pairing_heap
   by unfold_locales (rule hm_le hm_trans hm_transt hm_totalt)+
